Isabelle/Shelley/Ledger.thy
@@ -4,8 +4,32 @@ theory Ledger
   imports UTxO Delegation
 begin
 
+subsubsection \<open>Ledger transition-system types\<close>
+
+text \<open> Ledger environment \<close>
+
+type_synonym l_env = "
+  slot \<times> \<comment> \<open>current slot\<close>
+  ix \<times> \<comment> \<open>transaction index\<close>
+  p_params \<times> \<comment> \<open>protocol parameters\<close>
+  coin \<comment> \<open>total reserves\<close>"
+
 text \<open> Ledger state \<close>
 
 type_synonym l_state = "utxo_state \<times> d_p_state"
+
+text \<open> Ledger inference rule \<close>
+
+text \<open>
+  NOTE:
+  \<^item> \<open>stkCreds\<close>, \<open>stpools\<close> and \<open>genDelegs\<close> are not included for now.
+\<close>
+inductive ledger_sts :: "l_env \<Rightarrow> l_state \<Rightarrow> tx \<Rightarrow> l_state \<Rightarrow> bool"
+  (\<open>_ \<turnstile> _ \<rightarrow>\<^bsub>LEDGER\<^esub>{_} _\<close> [51, 0, 51] 50)
+  where
+    ledger: "
+      (slot, tx_ix, pp, reserves) \<turnstile> (utxo_st, dpstate) \<rightarrow>\<^bsub>LEDGER\<^esub>{tx} (utxo_st', dpstate')"
+      if "(slot, tx) \<turnstile> dpstate \<rightarrow>\<^bsub>DELEGS\<^esub>{txcerts tx} dpstate'"
+      and "(slot, pp, undefined, undefined, undefined) \<turnstile> utxo_st \<rightarrow>\<^bsub>UTXOW\<^esub>{tx} utxo_st'"
 
 end
